I now have one frac for each predicate. Instead of frac[this, OKP] and frac[this, ShareCountP] I have two global variables fracOKP[this] and fracShareCountP[this]

share1.bpl
@@ -1,10 +1,10 @@
 //class DoubleCount
 type Ref;
 type PredicateTypes;
-type FractionType = [Ref, PredicateTypes] int;
+type FractionType = [Ref] int;
 type PackedType = [Ref, PredicateTypes] bool;
 var packed: PackedType;
-var frac: FractionType;
+var fracOKP: FractionType;
 const null: Ref;
 
 var val: [Ref]int;
@@ -19,9 +19,9 @@ requires packed[this, OKP];
 ensures (dbl[this]==2*val[this]);
 
 procedure increment(this:Ref)
-modifies val, dbl, packed, frac;
-requires packed[this,OKP] && (frac[this,OKP] > 0);
-ensures packed[this,OKP] && (frac[this,OKP] > 0);
+modifies val, dbl, packed, fracOKP;
+requires packed[this,OKP] && (fracOKP[this] > 0);
+ensures packed[this,OKP] && (fracOKP[this] > 0);
 {
 call UnpackOK(this);
 packed[this, OKP]:=false;
@@ -35,28 +35,40 @@ packed[this, OKP]:=true;
 //class Share
 
 var dc: [Ref]Ref;
+var fracShareCountP: FractionType;
 
 const unique ShareCountP: PredicateTypes;
 
 //need to write the ShareCount constructor so that
 //we can use new for it
 
-//procedure ShareConstructor();
+//procedure ShareConstructor() returns sc:Ref;
 //ensures ;
 
 procedure PackShareCount(this:Ref);
-requires (packed[dc[this], OKP] && (frac[dc[this], OKP] >= 50));
+requires (packed[dc[this], OKP] && (fracOKP[dc[this]] > 0));
 
 procedure UnpackShareCount(this:Ref);
 requires packed[this, ShareCountP];
-ensures (packed[dc[this], OKP] && (frac[dc[this], OKP] >= 50));
+ensures (packed[dc[this], OKP] && (fracOKP[dc[this]] > 0));
 
 procedure touch(this: Ref)
-modifies val, dbl, packed, frac;
-requires packed[this, ShareCountP] && (frac[this, ShareCountP] > 0);
-ensures packed[this, ShareCountP] && (frac[this, ShareCountP] > 0);
+modifies val, dbl, packed, fracOKP, fracShareCountP;
+requires packed[this, ShareCountP] && (fracShareCountP[this] > 0);
+ensures packed[this, ShareCountP] && (fracShareCountP[this] > 0);
 {
+call UnpackShareCount(this);
+packed[this, ShareCountP]:=false;
+
+//assert packed[dc[this],OKP];
+//assert (frac[dc[this],OKP] > 0);
+assert (fracShareCountP[this] > 0);
 call increment(dc[this]) ;
+assert (fracShareCountP[this] > 0);
+call PackShareCount(this);
+packed[this, ShareCountP]:=true;
+assert packed[this, ShareCountP];
+assert (fracShareCountP[this] > 0);
 }
 
 //procedure main()
